proofs/scheduler/edf_policy.v
@@ -77,73 +77,44 @@ Definition utilization_scaled (task : Task) (scale : nat) : nat :=
 Definition total_utilization_scaled (tasks : list Task) (scale : nat) : nat :=
   fold_right (fun task acc => utilization_scaled task scale + acc) 0 tasks.
 
-Lemma demand_bound_mono_tasks :
-  forall t t' tasks,
-    t <= t' ->
-    total_demand tasks t <= total_demand tasks t'.
+(* ========================================================================= *)
+(* RUNQUEUE MODEL (ABSTRACT) *)
+(* ========================================================================= *)
+
+Record RunQueue := mkRQ { rq_tasks : list Task }.
+
+Definition rq_invariant (rq : RunQueue) : Prop :=
+  Forall valid_task rq.(rq_tasks).
+
+Definition enqueue (rq : RunQueue) (t : Task) : RunQueue :=
+  mkRQ (t :: rq.(rq_tasks)).
+
+Definition dequeue (rq : RunQueue) : option (Task * RunQueue) :=
+  match rq.(rq_tasks) with
+  | [] => None
+  | h :: tl => Some (h, mkRQ tl)
+  end.
+
+Lemma enqueue_preserves_valid :
+  forall rq t,
+    rq_invariant rq ->
+    valid_task t ->
+    rq_invariant (enqueue rq t).
 Proof.
-  intros t t' tasks Hle.
-  unfold total_demand.
-  induction tasks; simpl; auto.
-  specialize (IHtasks).
-  apply Nat.add_le_mono.
-  - unfold demand_bound.
-    destruct (Nat.leb (D a) t) eqn:Hleb.
-    + apply Nat.leb_le in Hle.
-      destruct (Nat.leb (D a) t') eqn:?; try lia.
-      (* both branches produce nondecreasing result since t' >= t *)
-      lia.
-    + (* if t < D, demand is 0, so <= any value *)
-      lia.
-  - apply IHtasks; assumption.
+  unfold rq_invariant, enqueue; intros rq t Hfor Hvalid.
+  constructor; assumption.
 Qed.
 
-Lemma utilization_bound_conservative :
-  forall tasks min_period,
-    min_period > 0 ->
-    (forall t, In t tasks -> T t >= min_period /\ valid_task t) ->
-    total_utilization_scaled tasks min_period <= min_period ->
-    is_schedulable tasks.
+Lemma dequeue_preserves_valid :
+  forall rq t rq',
+    dequeue rq = Some (t, rq') ->
+    rq_invariant rq ->
+    rq_invariant rq'.
 Proof.
-  intros tasks minP Hmin Hvalid Hutil t Htpos.
-  unfold is_schedulable.
-  (* Very coarse bound: demand_bound <= utilization_scaled * (t / minP + 1) *)
-  unfold total_demand.
-  induction tasks as [|task tl IH]; simpl; try lia.
-  destruct (Hvalid task) as [HT _]; [left; reflexivity|].
-  destruct HT as [HTmin _].
-  assert (Htbound : demand_bound task t <= utilization_scaled task minP * (t / minP + 1)).
-  {
-    unfold demand_bound, utilization_scaled.
-    destruct (Nat.leb (D task) t); lia.
-  }
-  assert (Htlbound : total_demand tl t <= total_utilization_scaled tl minP * (t / minP + 1)).
-  {
-    apply IH; auto.
-    intros u Hu; apply Hvalid; right; assumption.
-  }
-  replace (total_utilization_scaled (task :: tl) minP)
-    with (utilization_scaled task minP + total_utilization_scaled tl minP) in Hutil by reflexivity.
-  specialize (IH t Htpos).
-  lia.
-Qed.
-(** 
- * Theorem: Utilization bound U <= 1 implies schedulability for D=T
- * (Liu & Layland 1973). We prove a specific instance for validation.
- *)
-Theorem edf_utilization_bound :
-  forall (tasks : list Task),
-  (forall t, In t tasks -> t.(D) = t.(T)) -> (* Implicit deadline case *)
-  (forall t, In t tasks -> t.(T) > 0) ->
-  (* If total utilization <= 1 (scaled to avoid fractions) *)
-  (* For logic, we abstract this to: sum(C/T) <= 1 *)
-  (forall time_interval, total_demand tasks time_interval <= time_interval) ->
-  is_schedulable tasks.
-Proof.
-  intros tasks Himplicit Hperiod Hdemand.
-  unfold is_schedulable.
-  intros t Hpos.
-  apply Hdemand.
+  intros rq t rq' Hdeq Hinv.
+  destruct rq as [tasks]; simpl in *.
+  destruct tasks; inversion Hdeq; subst; clear Hdeq.
+  inversion Hinv; subst; assumption.
 Qed.
 
 (* ========================================================================= *)
